chore: use my upstream Parsec

LeanSAT/External/Parsec.lean
@@ -3,185 +3,279 @@ Copyright (c) 2024 Lean FRO, LLC. All rights reserved.
 Released under Apache 2.0 license as described in the file LICENSE.
 Authors: Henrik Böving
 -/
-namespace LRAT
 
-structure ByteArray.Iterator where
-  arr : ByteArray
-  pos : Nat
+namespace ByteArray
+
+/-- Iterator over the bytes (`UInt8`) of a `ByteArray`.
+
+Typically created by `arr.iter`, where `arr` is a `ByteArray`.
+
+An iterator is *valid* if the position `i` is *valid* for the array `arr`, meaning `0 ≤ i ≤ arr.size`
+
+Most operations on iterators return arbitrary values if the iterator is not valid. The functions in
+the `ByteArray.Iterator` API should rule out the creation of invalid iterators, with two exceptions:
+
+- `Iterator.next iter` is invalid if `iter` is already at the end of the array (`iter.atEnd` is
+  `true`)
+- `Iterator.forward iter n`/`Iterator.nextn iter n` is invalid if `n` is strictly greater than the
+  number of remaining bytes.
+-/
+structure Iterator where
+  /-- The array the iterator is for. -/
+  array : ByteArray
+  /-- The current position.
+
+  This position is not necessarily valid for the array, for instance if one keeps calling
+  `Iterator.next` when `Iterator.atEnd` is true. If the position is not valid, then the
+  current byte is `(default : UInt8)`. -/
+  idx : Nat
   deriving Inhabited
 
-namespace ByteArray.Iterator
+/-- Creates an iterator at the beginning of an array. -/
+def mkIterator (arr : ByteArray) : Iterator :=
+  ⟨arr, 0⟩
 
-def fresh (arr : ByteArray) : ByteArray.Iterator :=
-  { arr := arr, pos := 0 }
+@[inherit_doc mkIterator]
+abbrev iter := mkIterator
 
+/-- The size of an array iterator is the number of bytes remaining. -/
+instance : SizeOf Iterator where
+  sizeOf i := i.array.size - i.idx
+
+theorem Iterator.sizeOf_eq (i : Iterator) : sizeOf i = i.array.size - i.idx :=
+  rfl
+
+namespace Iterator
+
+/-- Number of bytes remaining in the iterator. -/
+def remainingBytes : Iterator → Nat
+  | ⟨arr, i⟩ => arr.size - i
+
+@[inherit_doc Iterator.idx]
+def pos := Iterator.idx
+
+/-- The byte at the current position.
+
+On an invalid position, returns `(default : UInt8)`. -/
 @[inline]
-def next (it : Iterator) : Iterator :=
-  let ⟨arr, pos⟩ := it
-  ⟨arr, pos + 1⟩
+def curr : Iterator → UInt8
+  | ⟨arr, i⟩ =>
+    if h:i < arr.size then
+      arr[i]'h
+    else
+      default
 
+/-- Moves the iterator's position forward by one byte, unconditionally.
+
+It is only valid to call this function if the iterator is not at the end of the array, *i.e.*
+`Iterator.atEnd` is `false`; otherwise, the resulting iterator will be invalid. -/
 @[inline]
-def curr (it : Iterator) : UInt8 :=
-  let ⟨arr, pos⟩ := it
-  if h:pos < arr.size then
-    arr[pos]'h
-  else
-    default
+def next : Iterator → Iterator
+  | ⟨arr, i⟩ => ⟨arr, i + 1⟩
 
+/-- Decreases the iterator's position.
+
+If the position is zero, this function is the identity. -/
 @[inline]
-def hasNext (it : Iterator) : Bool :=
-  let ⟨arr, pos⟩ := it
-  pos < arr.size
+def prev : Iterator → Iterator
+  | ⟨arr, i⟩ => ⟨arr, i - 1⟩
 
-end ByteArray.Iterator
+/-- True if the iterator is past the array's last byte. -/
+@[inline]
+def atEnd : Iterator → Bool
+  | ⟨arr, i⟩ => i ≥ arr.size
 
-inductive Parsec.ParseResult (α : Type) (s : Type) where
-  | success (pos : s) (res : α)
-  | error (pos : s) (err : String)
+/-- True if the iterator is not past the array's last byte. -/
+@[inline]
+def hasNext : Iterator → Bool
+  | ⟨arr, i⟩ => i < arr.size
+
+/-- True if the position is not zero. -/
+@[inline]
+def hasPrev : Iterator → Bool
+  | ⟨_, i⟩ => i > 0
+
+/-- Moves the iterator's position to the end of the array.
+
+Note that `i.toEnd.atEnd` is always `true`. -/
+@[inline]
+def toEnd : Iterator → Iterator
+  | ⟨arr, _⟩ => ⟨arr, arr.size⟩
+
+/-- Moves the iterator's position several bytes forward.
+
+The resulting iterator is only valid if the number of bytes to skip is less than or equal to
+the number of bytes left in the iterator. -/
+@[inline]
+def forward : Iterator → Nat → Iterator
+  | ⟨arr, i⟩, f => ⟨arr, i + f⟩
+
+@[inherit_doc forward, inline]
+def nextn : Iterator → Nat → Iterator := forward
+
+/-- Moves the iterator's position several bytes back.
+
+If asked to go back more bytes than available, stops at the beginning of the array. -/
+@[inline]
+def prevn : Iterator → Nat → Iterator
+  | ⟨arr, i⟩, f => ⟨arr, i - f⟩
+
+end Iterator
+end ByteArray
+
+namespace LRAT
+namespace Parsec
+
+inductive ParseResult (α : Type) (ι : Type) where
+  | success (pos : ι) (res : α)
+  | error (pos : ι) (err : String)
   deriving Repr
 
-def Parsec (s : Type) (α : Type) : Type := s → Parsec.ParseResult α s
+end Parsec
+
+def Parsec (ι : Type) (α : Type) : Type := ι → Parsec.ParseResult α ι
 
 namespace Parsec
 
-class Stream (s : Type) (elem : outParam Type) (idx : outParam Type) [DecidableEq idx] [ToString elem] [DecidableEq elem] where
-  pos : s → idx
-  next : s → s
-  curr : s → elem
-  hasNext : s → Bool
+class Input (ι : Type) (elem : outParam Type) (idx : outParam Type) [DecidableEq idx] [DecidableEq elem] where
+  pos : ι → idx
+  next : ι → ι
+  curr : ι → elem
+  hasNext : ι → Bool
 
-instance : Stream String.Iterator Char String.Pos where
-  pos it := it.pos
-  next it := it.next
-  curr it := it.curr
-  hasNext it := it.hasNext
+variable {α : Type} {ι : Type} {elem : Type} {idx : Type}
+variable [DecidableEq idx] [DecidableEq elem] [Input ι elem idx]
 
-instance : Stream ByteArray.Iterator UInt8 Nat where
-  pos it := it.pos
-  next it := it.next
-  curr it := it.curr
-  hasNext it := it.hasNext
-
-instance : Inhabited (Parsec s α) where
+instance : Inhabited (Parsec ι α) where
   default := fun it => .error it ""
 
 @[inline]
-protected def pure (a : α) : Parsec s α := fun it =>
- .success it a
+protected def pure (a : α) : Parsec ι α := fun it =>
+  .success it a
 
 @[inline]
-def bind (f : Parsec s α) (g : α → Parsec s β) : Parsec s β := λ it =>
+def bind {α β : Type} (f : Parsec ι α) (g : α → Parsec ι β) : Parsec ι β := fun it =>
   match f it with
   | .success rem a => g a rem
   | .error pos msg => .error pos msg
 
-instance : Monad (Parsec s) where
+instance : Monad (Parsec ι) where
   pure := Parsec.pure
-  bind := bind
+  bind := Parsec.bind
 
 @[inline]
-def fail (msg : String) : Parsec s α := fun it =>
+def fail (msg : String) : Parsec ι α := fun it =>
   .error it msg
 
-variable [DecidableEq idx] [ToString elem] [DecidableEq elem] [Stream s elem idx]
-
 @[inline]
-def tryCatch (p : Parsec s α)
-    (csuccess : α → Parsec s β)
-    (cerror : Unit → Parsec s β)
-    : Parsec s β := fun it =>
+def tryCatch (p : Parsec ι α) (csuccess : α → Parsec ι β) (cerror : Unit → Parsec ι β)
+    : Parsec ι β := fun it =>
   match p it with
   | .success rem a => csuccess a rem
   | .error rem err =>
-    if Stream.pos it = Stream.pos rem then cerror () rem else .error rem err
+    -- We assume that it.s never changes as the `Parsec` monad only modifies `it.pos`.
+    if Input.pos it = Input.pos rem then cerror () rem else .error rem err
 
 @[inline]
-def orElse (p : Parsec s α) (q : Unit → Parsec s α) : Parsec s α :=
+def orElse (p : Parsec ι α) (q : Unit → Parsec ι α) : Parsec ι α :=
   tryCatch p pure q
 
 @[inline]
-def attempt (p : Parsec s α) : Parsec s α := fun it =>
+def attempt (p : Parsec ι α) : Parsec ι α := fun it =>
   match p it with
   | .success rem res => .success rem res
   | .error _ err => .error it err
 
-instance : Alternative (Parsec s) where
+instance : Alternative (Parsec ι) where
   failure := fail ""
   orElse := orElse
-
-protected def run [Repr idx] (p : Parsec s α) (input : s) : Except String α :=
-  match p input with
-  | Parsec.ParseResult.success _ res => Except.ok res
-  | Parsec.ParseResult.error it err  => Except.error s!"offset {repr (Stream.pos it)}: {err}"
 
 def expectedEndOfInput := "expected end of input"
 
 @[inline]
-def eof : Parsec s Unit := fun it =>
-  if Stream.hasNext it then
+def eof : Parsec ι Unit := fun it =>
+  if Input.hasNext it then
     .error it expectedEndOfInput
   else
     .success it ()
 
 @[specialize]
-partial def manyCore (p : Parsec s α) (acc : Array α) : Parsec s (Array α) :=
+partial def manyCore (p : Parsec ι α) (acc : Array α) : Parsec ι <| Array α :=
   tryCatch p (manyCore p <| acc.push ·) (fun _ => pure acc)
 
 @[inline]
-def many (p : Parsec s α) : Parsec s (Array α) := manyCore p #[]
+def many (p : Parsec ι α) : Parsec ι <| Array α := manyCore p #[]
 
 @[inline]
-def many1 (p : Parsec s α) : Parsec s (Array α) := do manyCore p #[← p]
+def many1 (p : Parsec ι α) : Parsec ι <| Array α := do manyCore p #[← p]
 
 def unexpectedEndOfInput := "unexpected end of input"
 
 @[inline]
-def anyChar : Parsec s elem := fun it =>
-  if Stream.hasNext it then .success (Stream.next it) (Stream.curr it) else .error it unexpectedEndOfInput
+def any : Parsec ι elem := fun it =>
+  if Input.hasNext it then
+    .success (Input.next it) (Input.curr it)
+  else
+    .error it unexpectedEndOfInput
 
 @[inline]
-def pchar (c : elem) : Parsec s elem := attempt do
-  if (← anyChar) = c then pure c else fail s!"expected: '{c}'"
-
-@[inline]
-def skipElem (c : elem) : Parsec s Unit := pchar c *> pure ()
-
-@[inline]
-def satisfy (p : elem → Bool) : Parsec s elem := attempt do
-  let c ← anyChar
+def satisfy (p : elem → Bool) : Parsec ι elem := attempt do
+  let c ← any
   if p c then return c else fail "condition not satisfied"
 
 @[inline]
-def notFollowedBy (p : Parsec s α) : Parsec s Unit := fun it =>
+def notFollowedBy (p : Parsec ι α) : Parsec ι Unit := fun it =>
   match p it with
   | .success _ _ => .error it ""
   | .error _ _ => .success it ()
 
 @[inline]
-def peek? : Parsec s (Option elem) := fun it =>
-  if Stream.hasNext it then
-    .success it (Stream.curr it)
+def peek? : Parsec ι (Option elem) := fun it =>
+  if Input.hasNext it then
+    .success it (Input.curr it)
   else
     .success it none
 
 @[inline]
-def peek! : Parsec s elem := do
+def peek! : Parsec ι elem := do
   let some c ← peek? | fail unexpectedEndOfInput
   return c
 
 @[inline]
-def skip : Parsec s Unit := fun it =>
-  .success (Stream.next it) ()
+def skip : Parsec ι Unit := fun it =>
+  .success (Input.next it) ()
+
+@[specialize]
+partial def manyCharsCore (p : Parsec ι Char) (acc : String) : Parsec ι String :=
+  tryCatch p (manyCharsCore p <| acc.push ·) (fun _ => pure acc)
 
 @[inline]
-def eof? : Parsec s Bool := fun it =>
-  .success it (!Stream.hasNext it)
+def manyChars (p : Parsec ι Char) : Parsec ι String := manyCharsCore p ""
 
-namespace Byte
+@[inline]
+def many1Chars (p : Parsec ι Char) : Parsec ι String := do manyCharsCore p (← p).toString
+
+def eof? : Parsec ι Bool := fun it =>
+  .success it (!Input.hasNext it)
+
+namespace ByteArray
+
+instance : Input ByteArray.Iterator UInt8 Nat where
+  pos it := it.pos
+  next it := it.next
+  curr it := it.curr
+  hasNext it := it.hasNext
+
+abbrev Parser (α : Type) : Type := Parsec ByteArray.Iterator α
+
+protected def Parser.run (p : Parser α) (arr : ByteArray) : Except String α :=
+  match p arr.iter with
+  | .success _ res => Except.ok res
+  | .error it err  => Except.error s!"offset {repr it.pos}: {err}"
 
 @[inline]
 def digit : Parsec ByteArray.Iterator UInt8 := attempt do
-  let c ← anyChar
+  let c ← any
   if '0'.toNat.toUInt8 ≤ c ∧ c ≤ '9'.toNat.toUInt8 then return c else fail s!"digit expected"
 
 @[inline]
@@ -216,15 +310,58 @@ def digits : Parsec ByteArray.Iterator Nat := do
   digitsCore (digitToNat d)
 
 @[inline]
-def skipChar (c : Char) : Parsec ByteArray.Iterator Unit := pchar c.toNat.toUInt8 *> pure ()
+def pbyte (b : UInt8) : Parser UInt8 := attempt do
+  if (← any) = b then pure b else fail s!"expected: '{b}'"
 
-def skipString (s : String) : Parsec ByteArray.Iterator Unit := do
-  let arr := s.toUTF8
-  for byte in arr do
-    skipElem byte
+@[inline]
+def skipByte (b : UInt8) : Parser Unit := pbyte b *> pure ()
 
-end Byte
+def skipBytes (arr : ByteArray) : Parser Unit := do
+  for b in arr do
+    skipByte b
 
+@[inline]
+def pstring (s : String) : Parser String := do
+  skipBytes s.toUTF8
+  return s
+
+@[inline]
+def skipString (s : String) : Parser Unit := pstring s *> pure ()
+
+/--
+Parse a `Char` that can be represented in 1 byte. If `c` uses more than 1 byte it is truncated.
+-/
+@[inline]
+def pByteChar (c : Char) : Parser Char := attempt do
+  if (← any) = c.toUInt8 then pure c else fail s!"expected: '{c}'"
+
+/--
+Skip a `Char` that can be represented in 1 byte. If `c` uses more than 1 byte it is truncated.
+-/
+@[inline]
+def skipByteChar (c : Char) : Parser Unit := skipByte c.toUInt8
+
+private partial def skipWs (it : ByteArray.Iterator) : ByteArray.Iterator :=
+  if it.hasNext then
+    let b := it.curr
+    if b = '\u0009'.toUInt8 ∨ b = '\u000a'.toUInt8 ∨ b = '\u000d'.toUInt8 ∨ b = '\u0020'.toUInt8 then
+      skipWs it.next
+    else
+      it
+  else
+   it
+
+@[inline]
+def ws : Parser Unit := fun it =>
+  .success (skipWs it) ()
+
+def take (n : Nat) : Parser ByteArray := fun it =>
+  let subarr := it.array.extract it.idx (it.idx + n)
+  if subarr.size != n then
+    .error it s!"expected: {n} bytes"
+  else
+    .success (it.forward n) subarr
+
+end ByteArray
 end Parsec
-
 end LRAT
